theories/clang/notations.v
@@ -2,7 +2,6 @@ From iris_c.clang Require Import lang.
 Set Default Proof Using "Type".
 
 Coercion Vint8 : int8 >-> val.
-(* Coercion Vint32 : int32 >-> val. *)
 Coercion Vptr : addr >-> val.
 Coercion Evalue : val >-> expr.
 Coercion Evar : string >-> expr.
@@ -11,7 +10,7 @@ Notation "'void'" := Vvoid.
 Notation "'null'" := Vnull.
 Notation "# v" := (Evalue v) (at level 8) : expr_scope.
 Notation "!? e" := (Ederef e%E) (at level 9, right associativity) : expr_scope.
-Notation "! e @ t" := (Ederef_typed t e%E) (at level 9, right associativity) : expr_scope.
+Notation "! e @ t" := (Ederef t e%E) (at level 9, right associativity) : expr_scope.
 Notation "'fst' e" := (Efst e%E) (at level 9, right associativity) : expr_scope.
 Notation "'snd' e" := (Esnd e%E) (at level 9, right associativity) : expr_scope.
 Notation "& e" := (Eaddrof e%E)
@@ -36,7 +35,3 @@ Notation "'while:' ( e ) ( s ) " := (Ewhile e%E s%E)
 Notation "s1 ;; s2" := (Eseq s1%E s2%E)
   (at level 100, s2 at level 200, format "s1  ;;  s2") : expr_scope.
 Notation "'return:' e" := (Erete e%E) (at level 80): expr_scope.
-(* Notation "'let:' x ::: t := e1 'in' e2" := (Elet t x e1%E e2%E) *)
-(*   (at level 102, x, t at level 1, e1, e2 at level 200) : expr_scope. *)
-(* Notation "'let:' x ::: t 'in' e2" := (Edecl t x e2%E) *)
-(*   (at level 102, x, t at level 1, e2 at level 200) : expr_scope. *)
