README.md
@@ -3,7 +3,7 @@ Iris C
 
 [![Build Status](https://travis-ci.org/izgzhen/iris-c-coq.svg?branch=master)](https://travis-ci.org/izgzhen/iris-c-coq)
 
-C verification framework based on the Iris program logic.
+Control-flow based language verification framework based on the Iris program logic.
 
 [Example](theories/tests/swap.v)
 
